Move general-purpose definitions out of Subparser

AllStar/Subparser.v
@@ -1,5 +1,5 @@
 Require Import Bool List Omega String Program.Wf.
-Require Import Grammar Lib.Utils Lib.Tactics.
+Require Import Grammar Lib.Lemmas Lib.Tactics Lib.Utils.
 Import ListNotations.
 Open Scope string_scope.
 
@@ -27,156 +27,45 @@ Definition move (token : string)
       end 
   in  concat (map moveSp sps).
 
-Definition removeOpt (x : symbol) (s : SymbolSet.t) :=
-  if SymbolSet.mem x s then Some (SymbolSet.remove x s) else None.
-
-Lemma empty_nil : forall s,
-    SymbolSet.Empty s <-> SymbolSet.elements s = [].
-Proof. 
-  intros; split; intros.
-  - destruct (SymbolSet.elements s) as [| e es] eqn:Hs.
-    + reflexivity.
-    + exfalso. 
-      unfold SymbolSet.Empty in H; eapply H; clear H.
-      assert (SetoidList.InA eq e (SymbolSet.elements s)).
-      { rewrite Hs; constructor; reflexivity. }
-      eapply SymbolSetFacts.elements_iff. eassumption.
-  - unfold SymbolSet.Empty; unfold not; intros e Hin.
-    rewrite SymbolSetFacts.elements_iff in Hin. 
-    rewrite H in Hin. inv Hin.
-Qed.
-
-Lemma list_remove_le : forall (x : symbol) (ys : list symbol),
-    List.length (remove symbol_eq_dec x ys) <= List.length ys.
-Proof.
-  intros. induction ys as [| y ys]; simpl.
-  - reflexivity.
-  - destruct (symbol_eq_dec x y); simpl; omega.
-Qed.
-
-Lemma list_remove_lt : forall (x : symbol) (ys : list symbol),
-    List.In x ys -> 
-    List.length (remove symbol_eq_dec x ys) < List.length ys.
-Proof.
-  intros. induction ys as [| y ys]; simpl.
-  - inv H.
-  - destruct (symbol_eq_dec x y) as [Heq | Hneq]; simpl.
-    + pose proof list_remove_le as Hle.
-      specialize Hle with (x := x) (ys := ys). omega.
-    + apply lt_n_S. apply IHys. clear IHys.
-      simpl in H. destruct H as [Hhd | Htl].
-      * exfalso. apply Hneq. symmetry. assumption.
-      * assumption.
-Qed.
-
-Lemma cardinal_length : forall s s',
-    SymbolSet.cardinal s' < SymbolSet.cardinal s <-> 
-    List.length (SymbolSet.elements s') < List.length (SymbolSet.elements s).
-Proof.
-  intros. split; intros.
-  - repeat rewrite <- SymbolSet.cardinal_spec. assumption.
-  - repeat rewrite SymbolSet.cardinal_spec. assumption.
-Qed.
-
-Lemma remove_not_In : forall x ys,
-    ~In x ys <-> remove symbol_eq_dec x ys = ys.
-Proof.
-  intros; split; unfold not; intros.
-  - induction ys; simpl.
-    + reflexivity.
-    + destruct (symbol_eq_dec x a); simpl.
-      * exfalso. subst. apply H. apply in_eq.
-      * assert (Htls : remove symbol_eq_dec x ys = ys).
-      { apply IHys; intros; clear IHys.
-        apply H. apply in_cons. assumption. }
-      rewrite Htls; reflexivity.
-  - rewrite <- H in H0. eapply remove_In. eassumption.
-Qed.             
-
-(* HERE is the lemma I needed -- wish I'd found remove_cardinal_1 sooner...*)
-Lemma removeOptDecreasing : forall (x : symbol) (s s' : SymbolSet.t),
-    removeOpt x s = Some s' ->
-    SymbolSet.cardinal s' < SymbolSet.cardinal s.
-Proof.
-  intros. unfold removeOpt in H. 
-  destruct (SymbolSet.mem x s) eqn:Hmem.
-  - inv H.
-    pose proof SymbolSetEqProps.remove_cardinal_1.
-    apply H in Hmem. omega.
-  - inv H.
-Qed.
-
-(* if removeOpt x l  = Some l', l' is a sublist of l *)
-Fixpoint removeOpt' {A} (x : A) (l : list A) (beq : A -> A -> bool) :=
-  match l with
-  | nil => None
-  | y :: l' => 
-    if beq x y then
-      Some l'
-    else
-      match removeOpt' x l' beq with
-      | None => None
-      | Some l'' => Some (y :: l'')
-      end
+(* Advance a single subparser as far as possible without
+   consuming an input symbol *)
+Program Fixpoint spClosure
+        (g : grammar) (freeSyms : SymbolSet.t) (sp : subparser)
+        {measure (SymbolSet.cardinal freeSyms)}
+        : list subparser :=
+  match sp.(stack) with
+  | nil => [sp]
+  | T _ :: _ => [sp]
+  | NT x :: stack' => 
+    match removeOpt (NT x) freeSyms with
+    | None => nil (* recursion detected *)
+    | Some freeSyms' =>
+      let newSps :=
+          map (fun gamma => mkSp (gamma ++ stack') sp.(pred))
+              (rhss g x)
+      in  concat (map (fun sp => spClosure g freeSyms' sp)
+                      newSps)
+    end
   end.
-
-(* ... and here's the proof: *)
-Lemma removeOpt'Decreasing : forall A (x : A) beq (ys zs : list A),
-    removeOpt' x ys beq = Some zs ->
-    List.length zs < List.length ys.
-Proof.
-  induction ys as [| y ys]; intros zs H.
-  - inversion H.
-  - simpl in H.
-    destruct (beq x y).
-    + inv H; simpl; omega.
-    + destruct (removeOpt' x ys beq).
-      * inv H. simpl.
-        apply lt_n_S; apply IHys; reflexivity.
-      * inv H.
-Qed.
-
-Program Fixpoint spClosure (g : grammar)
-                           (freeSyms : list symbol)
-                           (sp : subparser) 
-                           {measure (List.length freeSyms)}
-                           : list subparser :=
-       match sp.(stack) with
-       | nil => [sp]
-       | T _ :: _ => [sp]
-       | NT x :: stack' => 
-         match removeOpt' (NT x) freeSyms beqSym with
-         | None => nil (* recursion detected *)
-         | Some freeSyms' => 
-           concat (map (fun gamma => 
-                          spClosure g freeSyms' (mkSp (gamma ++ stack') sp.(pred)))
-                       (rhss g x))
-         end
-       end.
 Obligation 1.
-eapply removeOpt'Decreasing. symmetry. eassumption.
+eapply removeOptDecreasing. symmetry. eassumption.
 Qed.
 
-Definition nonterminals g :=
-  let prodNTs p :=
-      match p with
-      | (l, rs) => l :: filter isNT rs
-      end
-  in  concat (map prodNTs g).
-
-Definition closure (g : grammar) 
-                   (freeSyms : list symbol) 
-                   (sps : list subparser)
-                   : list subparser :=
+Definition closure
+           (g : grammar) (freeSyms : SymbolSet.t)
+           (sps : list subparser) : list subparser :=
   concat (map (spClosure g freeSyms) sps).
 
 (* LL predict when stack0 is nil, SLL predict otherwise *)
 Definition startState g x stack0 :=
   let sps := map (fun gamma =>
-                    mkSp (gamma ++ stack0) gamma) (rhss g x)
+                    mkSp (gamma ++ stack0) gamma)
+                 (rhss g x)
   in  closure g (nonterminals g) sps.
 
-Definition target g sps (token : string) :=
+Definition target
+           (g : grammar) (sps : list subparser)
+           (token : string) : list subparser :=
   closure g (nonterminals g) (move token sps).
 
 Fixpoint conflict sps : bool :=
@@ -221,7 +110,8 @@ Definition adaptivePredict g x input stack0 :=
       | _ => sllPred
       end.
 
-
+(* Here's the beginning of another way to prove termination
+   based on the length of a list *)
 Section lengthorder.
   Variable A : Type.
   
@@ -243,4 +133,3 @@ Section lengthorder.
   Defined.
   
 End lengthorder.
-
