Lib/Lemmas.v
@@ -1,5 +1,5 @@
-Require Import Bool List String.
-Require Import Grammar Tactics Utils.
+Require Import Bool List Omega String.
+Require Import Grammar Lib.Tactics Lib.Utils.
 
 Lemma find_In : forall k vT (v : vT) m,
     SymbolMap.find k m = Some v ->
@@ -7,7 +7,7 @@ Lemma find_In : forall k vT (v : vT) m,
 Proof.
   intros. rewrite SymbolMapFacts.in_find_iff. rewrite H.
   unfold not. intro Hcontra. inv Hcontra.
-Defined.
+Qed.
 
 Ltac copy_and_find_In H :=
   let Hfind := fresh "Hfind" in
@@ -28,7 +28,7 @@ Proof.
     + rewrite H0 in H. inv H.
     + apply IHgamma with (y := y) in H1.
       apply H1. apply H0.
-Defined.
+Qed.
 
 (* Some useful lemmas to remember : in_eq, in_cons *)
 Lemma NT_list_neq_list_with_T :
@@ -42,7 +42,7 @@ Proof.
   apply H. clear H.
   rewrite H0. rewrite in_app_iff.
   right. apply in_eq.
-Defined.
+Qed.
 
 Lemma NT_not_in_T_list :
   forall (gamma : list symbol) (X : string),
@@ -57,7 +57,7 @@ Proof.
     + rewrite H0 in H. inv H.
     + apply IHgamma with (X := X) in H1.
       apply H1. assumption.
-Defined.
+Qed.
 
 Lemma T_list_neq_list_with_NT :
   forall (gamma prefix suffix : list symbol)
@@ -70,5 +70,82 @@ Proof.
   apply H; clear H.
   rewrite H0. rewrite in_app_iff.
   right. apply in_eq.
-Defined.
+Qed.
 
+(* A bunch of list and set lemmas that I probably won't need *)
+
+Lemma empty_nil : forall s,
+    SymbolSet.Empty s <-> SymbolSet.elements s = nil.
+Proof. 
+  intros; split; intros.
+  - destruct (SymbolSet.elements s) as [| e es] eqn:Hs.
+    + reflexivity.
+    + exfalso. 
+      unfold SymbolSet.Empty in H; eapply H; clear H.
+      assert (SetoidList.InA eq e (SymbolSet.elements s)).
+      { rewrite Hs; constructor; reflexivity. }
+      eapply SymbolSetFacts.elements_iff. eassumption.
+  - unfold SymbolSet.Empty; unfold not; intros e Hin.
+    rewrite SymbolSetFacts.elements_iff in Hin. 
+    rewrite H in Hin. inv Hin.
+Qed.
+
+Lemma list_remove_le : forall (x : symbol) (ys : list symbol),
+    List.length (remove symbol_eq_dec x ys) <= List.length ys.
+Proof.
+  intros. induction ys as [| y ys]; simpl.
+  - reflexivity.
+  - destruct (symbol_eq_dec x y); simpl; omega.
+Qed.
+
+Lemma list_remove_lt : forall (x : symbol) (ys : list symbol),
+    List.In x ys -> 
+    List.length (remove symbol_eq_dec x ys) < List.length ys.
+Proof.
+  intros. induction ys as [| y ys]; simpl.
+  - inv H.
+  - destruct (symbol_eq_dec x y) as [Heq | Hneq]; simpl.
+    + pose proof list_remove_le as Hle.
+      specialize Hle with (x := x) (ys := ys). omega.
+    + apply lt_n_S. apply IHys. clear IHys.
+      simpl in H. destruct H as [Hhd | Htl].
+      * exfalso. apply Hneq. symmetry. assumption.
+      * assumption.
+Qed.
+
+Lemma cardinal_length : forall s s',
+    SymbolSet.cardinal s' < SymbolSet.cardinal s <-> 
+    List.length (SymbolSet.elements s') < List.length (SymbolSet.elements s).
+Proof.
+  intros. split; intros.
+  - repeat rewrite <- SymbolSet.cardinal_spec. assumption.
+  - repeat rewrite SymbolSet.cardinal_spec. assumption.
+Qed.
+
+Lemma remove_not_In : forall x ys,
+    ~In x ys <-> remove symbol_eq_dec x ys = ys.
+Proof.
+  intros; split; unfold not; intros.
+  - induction ys; simpl.
+    + reflexivity.
+    + destruct (symbol_eq_dec x a); simpl.
+      * exfalso. subst. apply H. apply in_eq.
+      * assert (Htls : remove symbol_eq_dec x ys = ys).
+      { apply IHys; intros; clear IHys.
+        apply H. apply in_cons. assumption. }
+      rewrite Htls; reflexivity.
+  - rewrite <- H in H0. eapply remove_In. eassumption.
+Qed.             
+
+Lemma removeOptDecreasing :
+  forall (x : symbol) (s s' : SymbolSet.t),
+    removeOpt x s = Some s' ->
+    SymbolSet.cardinal s' < SymbolSet.cardinal s.
+Proof.
+  intros. unfold removeOpt in H. 
+  destruct (SymbolSet.mem x s) eqn:Hmem.
+  - inv H.
+    pose proof SymbolSetEqProps.remove_cardinal_1.
+    apply H in Hmem. omega.
+  - inv H.
+Qed.
